---
aspectratio: 169
author: D. Zack Garza
colortheme: default
date: April 2020
fontfamily: noto-sans
fontsize: 10pt
header-includes:
- |
  ```{=tex}
  \usepackage{cmbright}
  ```
subtitle: Section 8.4 Follow-Up
theme: Berkeley
title: Linearization Continued
---

```{=tex}
\usepackage{cmbright}
```

-   [Review](#review)
    -   [Definitions](#definitions)
    -   [The Frame](#the-frame)
    -   [Charts](#charts)
    -   [Add a Tangent](#add-a-tangent)
-   [8.4.1: Leibniz Rule](#leibniz-rule)
    -   [Leibniz Rule](#leibniz-rule-1)
    -   [Order 1](#order-1)
-   [Order 0 Part is Symmetric in the Limit](#order-0-part-is-symmetric-in-the-limit)
    -   [8.4.4: Order 0 Part is Symmetric in the Limit](#order-0-part-is-symmetric-in-the-limit-1)
    -   [Proof](#proof)
    -   [Proof: Blue Term Vanishes](#proof-blue-term-vanishes)
    -   [Proof: Orange Term Vanishes (1 and 3)](#proof-orange-term-vanishes-1-and-3)
    -   [Proof: Symmetry](#proof-symmetry)
    -   [Proof: Symmetry](#proof-symmetry-1)
    -   [Proof: Symmetry](#proof-symmetry-2)
    -   [Proof: Symmetry](#proof-symmetry-3)
-   [Lemma That Concludes the Proof](#lemma-that-concludes-the-proof)
    -   [Lemma](#lemma)
    -   [Proof of Lemma](#proof-of-lemma)
    -   [Proof of Lemma](#proof-of-lemma-1)
-   [8.4.6: Linearization of Hamilton's Equation](#linearization-of-hamiltons-equation)
    -   [Linearization of Hamilton's Equation](#linearization-of-hamiltons-equation-1)
    -   [Proof](#proof-1)
    -   [Proof](#proof-2)
    -   [Proof](#proof-3)














[[Floer Reading Group Fall 2020 | ../../../../Unsorted/Floer%20Reading%20Group%20Fall%202020.html]]

# Review

## Definitions

-   The Floer equation is given by `\begin{align*}
    \frac{\partial u}{\partial s}+J(u) \frac{\partial u}{\partial t}+\operatorname{grad} H_{t}(u)=0
    .\end{align*}`{=tex}

-   We fixed a solution and lifted it to a sphere: `
    <span class="math display">
    \begin{align*}
    u \in C^\infty(S^1\times{\mathbb{R}}; W) \quad\mapsto\quad \tilde u \in C^\infty(S^2; W) 
    \end{align*}
    <span>`{=html}

-   We use the assumption:

    > For every $w\in C^\infty(S^2, W)$ there exists a symplectic trivialization of the fiber bundle $w^* TW$, i.e.Â ${\left\langle {c_1(TW)},~{\pi_2(W)} \right\rangle} = 0$ where $c_1$ denotes the first Chern class of the bundle $TW$.

-   We use this trivialize the pullback $\tilde u ^* TW$ to obtain an orthonormal unitary frame `
    <span class="math display">
    \begin{align*}\left\{{Z_i}\right\}_{i=1}^{2n} \subset T_{u(s, t)} W\end{align*}
    <span>`{=html}

## The Frame

-   We used the chosen frame $\left\{{Z_i}\right\}$ to define a chart centered at $u$ of ${\mathcal{P}}^{1, p}(x, y)$ given by `\begin{align*}
    \iota: W^{1, p}\left(\mathbb{R} \times S^{1} ; \mathbb{R}^{2 n}\right) & \longrightarrow \mathcal{P}^{1, p}(x, y) \\
    Y = \left(y_{1}, \dots, y_{2 n}\right) & \longmapsto \exp _{u}\left(\sum y_{i} Z_{i}\right)
    .\end{align*}`{=tex}

-   We regard $Y(s, t)$ as a tangent vector to $W$ in some Euclidean embedding.

## Charts

-   We seek to compute the composite map in charts:

```{=tex}
\begin{center}
\includegraphics[height= 0.5\textheight]{figures/image_2020-04-16-01-11-02.png} 
\end{center}
```
## Add a Tangent

```{=tex}
\begin{center}
\begin{tikzcd}[ampersand replacement=\&, matrix scale=0.002]
{\mathcal{F}}(u) =
\& \frac{\partial u}{\partial s} 
\& + J(u) \frac{\partial u}{\partial t} 
\& - J(u)X_{t}(u) \\
\mathcal{F}(u+Y) =
\& \frac{\partial(u+Y)}{\partial s}
\&+ J(u+Y) \frac{\partial(u+Y)}{\partial t}
\&- J(u+Y) X_{t}(u+Y)
\end{tikzcd}
\end{center}
```
Extract the part that is linear in $Y$ and collect terms:

`\begin{align*}
&(d \mathcal{F})_{u}(Y)  \\
& = {\color{red}\frac{\partial Y}{\partial s}} +(d J)_{u}(Y) \frac{\partial u}{\partial t} + {\color{red} J(u) \frac{\partial Y}{\partial t}} -(d J)_{u}(Y) X_{t}-J(u)\left(d X_{t}\right)_{u}(Y) \\ 
& = 
\qty{ {\color{red}\frac{\partial Y}{\partial s}} + {\color{red} J(u) \frac{\partial Y}{\partial t}}}  \\
& \hspace{2em} + \qty{ (d J)_{u}(Y) \frac{\partial u}{\partial t} - (d J)_{u}(Y) X_{t}-J(u)\left(d X_{t}\right)_{u}(Y)} \\
.\end{align*}`{=tex}

# 8.4.1: Leibniz Rule

## Leibniz Rule

Recall the Leibniz rule `
<span class="math display">
\begin{align*}(dJ)(Y) \cdot v = d(Jv)(Y) - J dv(Y)\end{align*}
<span>`{=html} `\begin{align*}
(d \mathcal{F})_{u}(Y)
& = 
\qty{ {\color{red}\frac{\partial Y}{\partial s}} + {\color{red} J(u) \frac{\partial Y}{\partial t}}}  \\
& \quad + \qty{ (d J)_{u}(Y) \frac{\partial u}{\partial t} - (d J)_{u}(Y) X_{t}-J(u)\left(d X_{t}\right)_{u}(Y)} \\ 
&= \sum_{i=1}^{2n} \qty{ {\frac{\partial y_i}{\partial s}\,} Z_i + {\frac{\partial y_i}{\partial t}\,} J(u) Z_i} \\
& + \sum_{i=1}^{2n} y_i \Bigg( {\frac{\partial Z_i}{\partial s}\,} + J(u) {\frac{\partial Z_i}{\partial t}\,} + (dJ)_u (Z_i) {\frac{\partial u}{\partial t}\,}  \\
&\hspace{5em}- J(u) (dX_t)_u Z_i - (dJ)_u (Z_i) X_t \Bigg)
.\end{align*}`{=tex}

Use the fact that this is $O_1 + O_0$ in $Y$.

## Order 1

Study $O_1$ first, which (claim) reduces to `\begin{align*}
  O_1 = \sum_{i=1}^{2n} \qty{{\frac{\partial y_i}{\partial s}\,} + J_0 {\frac{\partial y_i}{\partial t}\,}  }Z_i = \mkern 1.5mu\overline{\mkern-1.5mu{\partial}\mkern-1.5mu}\mkern 1.5mu(y_1, \cdots, y_{2n})
  .\end{align*}`{=tex} where $J_0$ is the standard complex structure on ${\mathbb{R}}^{2n} = {\mathbb{C}}^n$

Use this to write `\begin{align*}
(d{\mathcal{F}})_u &= {\color{red} \mkern 1.5mu\overline{\mkern-1.5mu{\partial}\mkern-1.5mu}\mkern 1.5muY} + SY
\end{align*}`{=tex} where $S\in C^\infty({\mathbb{R}}\times S^1; \endo({\mathbb{R}}^n))$ is a linear operator of order 0.

# Order 0 Part is Symmetric in the Limit

## 8.4.4: Order 0 Part is Symmetric in the Limit

Theorem (8.4.4, CR + Symmetric in the Limit)

:   If $u$ solves Floer's equation, then `
    <span class="math display">
    \begin{align*}
    (d{\mathcal{F}})_u = \mkern 1.5mu\overline{\mkern-1.5mu{\partial}\mkern-1.5mu}\mkern 1.5mu+ S( s, t)
    \end{align*}
    <span>`{=html} where

    1.  $S$ is linear
    2.  $S$ tends to a symmetric operator as $s\to \pm \infty$, and
    3.  We have the limiting behavior `
        <span class="math display">
        \begin{align*}{\frac{\partial S}{\partial s}\,}(s, t)  \overset{s\to\pm\infty}\to 0 {\quad \operatorname{uniformly in $t$} \quad}\end{align*}
        <span>`{=html}

## Proof

Collect terms in the order zero part: `\begin{align*}
O_0 = S(y_1, \cdots , y_{2n}) 
&= \sum_{i=1}^{2n} y_i \Bigg[ {\color{orange} {\frac{\partial Z_i}{\partial s}\,}} + J(u) {\frac{\partial Z_i}{\partial t}\,} + {\color{blue} (dJ)_u (Z_i) {\frac{\partial u}{\partial t}\,}}  \\
&\hspace{5em}  - J(u) (dX_t)_u Z_i - {\color{blue} (dJ)_u (Z_i) X_t} \Bigg] \\
&= \sum_{i=1}^{2n} y_i \Bigg[ {\color{orange} {\frac{\partial Z_i}{\partial s}\,} } + { \color{blue} (dJ)_u (Z_i) \qty{ {\frac{\partial u}{\partial t}\,} - (Z_i) X_t} } \\
&\hspace{5em} + {\color{red} J(u) {\frac{\partial Z_i}{\partial t}\,}  - J(u) (dX_t)_u Z_i} \Bigg]
.\end{align*}`{=tex}

-   Claim: the terms in blue and orange vanish in the limit $s \to \pm \infty$, so it suffices to prove that the red term limits to a symmetric operator.

## Proof: Blue Term Vanishes

`
<span class="math display">
\begin{align*}
{ \color{blue} (dJ)_u (Z_i) \qty{ {\frac{\partial u}{\partial t}\,} - (Z_i) X_t} } \to 0
\end{align*}
<span>`{=html}

The term in blue vanishes: since $u$ is a solution and

`
<span class="math display">
\begin{align*}{\frac{\partial u}{\partial s}\,} \overset{s\to \pm \infty}\to 0 {\quad \operatorname{uniformly} \quad}\end{align*}
<span>`{=html}

as do its derivatives, we have

`
<span class="math display">
\begin{align*} \qty{ {\frac{\partial u}{\partial t}\,} - X_t(u)} \overset{s\to \pm\infty}\to 0 \end{align*}
<span>`{=html}

> This seems to be the full argument for the blue term.

## Proof: Orange Term Vanishes (1 and 3)

`
<span class="math display">
\begin{align*}
{\color{orange} {\frac{\partial Z_i}{\partial s}\,} } \overset{s\to \pm \infty}\to 0 
\end{align*}
<span>`{=html}

Follows since the frame $Z_i$ was chosen such that

`
<span class="math display">
\begin{align*}{\frac{\partial }{\partial s}\,}, \quad \frac{{\partial}^2}{{\partial}s^2}, \quad \frac{{\partial}^2}{{\partial}s~{\partial}t} \quad \curvearrowright Z_i \overset{s\to \pm\infty}\to 0\quad \text{for each } i\end{align*}
<span>`{=html}

This also implies

`
<span class="math display">
\begin{align*} {\frac{\partial S}{\partial s}\,} \overset{s\to \pm\infty}\to 0.\end{align*}
<span>`{=html}

> This shows parts (1) and (3) of the theorem: linearity and limits to zero uniformly in $t$?

## Proof: Symmetry

Write the remaining red term as

`\begin{align*}
A \coloneqq A\left(y_{1}, \ldots, y_{2 n}\right)=\sum y_{i}\left( {\color{red} J(u) \frac{\partial Z_{i}}{\partial t}-J(u)\left(d X_{t}\right)_{u}\left(Z_{i}\right) } \right)
.\end{align*}`{=tex}

Extract the $j$th component: `\begin{align*}
A_j = \sum y_{i}\left\langle J(u) \frac{\partial Z_{i}}{\partial t}-J(u)\left(d X_{t}\right)_{u}\left(Z_{i}\right), \quad Z_{j}\right\rangle
.\end{align*}`{=tex}

We'll show that `\begin{align*}
\lim _{s \rightarrow \pm \infty}
&\left\langle J(u) \frac{\partial Z_{\color{red} i}}{\partial t}-J(u)\left(d X_{t}\right)_{u}\left(Z_{\color{red} i}\right), Z_{\color{red} j}\right\rangle \\
- &\left\langle J(u) \frac{\partial Z_{\color{red} j}}{\partial t}-J(u)\left(d X_{t}\right)_{u} Z_{\color{red}j}, ~~~Z_{\color{red} i}\right\rangle=0
.\end{align*}`{=tex}

## Proof: Symmetry

Use the fact that the frame $\left\{{Z_i}\right\}$ is unitary: `\begin{align*}
0 &=\frac{\partial}{\partial t}\left\langle J(u) Z_{i}, Z_{j}\right\rangle \\
&=\left\langle(d J)_{u}\left(\frac{\partial u}{\partial t}\right) Z_{i}, Z_{j}\right\rangle+\left\langle J(u) \frac{\partial Z_{i}}{\partial t}, Z_{j}\right\rangle+\left\langle {\color{red} J(u) } Z_{i}, \frac{\partial Z_{j}}{\partial t}\right\rangle \\
&=
\left\langle(d J)_{u}\left(\frac{\partial u}{\partial t}\right) Z_{i}, Z_{j}\right\rangle+\left\langle J(u) \frac{\partial Z_{i}}{\partial t}, Z_{j}\right\rangle-\left\langle Z_{i}, {\color{red} J(u)} \frac{\partial Z_{j}}{\partial t}\right\rangle
.\end{align*}`{=tex}

## Proof: Symmetry

Therefore it suffices to show `\begin{align*}
-&\left\langle J(u)\left(d X_{t}\right)_{u}\left(Z_{i}\right), \quad Z_{j}\right\rangle \\
+&\left\langle J(u)\left(d X_{t}\right)_{u}\left(Z_{j}\right), \quad Z_{i}\right\rangle \\
-&\left\langle(d J)_{u}\left(\frac{\partial u}{\partial t}\right) Z_{i}, \quad Z_{j}\right\rangle \\ \\
&\overset{s\to \pm\infty}\to 0
.\end{align*}`{=tex}

## Proof: Symmetry

Using the fact that `\begin{align*}
\qty{ {\frac{\partial u}{\partial t}\,} - X_t(u)} \overset{s\to \pm\infty}\to 0
\end{align*}`{=tex}

we can equivalently show `\begin{align*}
&- \left\langle J(u)\left(d X_{t}\right)_{u}\left(Z_{i}\right), \quad Z_{j}\right\rangle \\
&+ \left\langle J(u)\left(d X_{t}\right)_{u} \left(Z_{j}\right), \quad Z_{i}\right\rangle \\
&- \left\langle(d J)_{u}\left(X_{t}\right) Z_{i}, \hspace{2.5em} Z_{j}\right\rangle \\ \\
&\overset{s\to \pm\infty}\to 0
\end{align*}`{=tex}

> For a fixed $(s, t)$, this expression only depends on $Z_i$ at the point $u(s, t)$.

# Lemma That Concludes the Proof

## Lemma

**Lemma**: For $p\in W$, $\left\{{Z_i}\right\}$ a unitary basis of $T_p W$, `\begin{align*}
&- \left\langle J(p)\left(d X_{t}\right)_{p}\left(Z_{i}\right), \quad Z_{j}\right\rangle \\
&+ \left\langle J(p)\left(d X_{t}\right)_{p}\left(Z_{j}\right), \quad Z_{i}\right\rangle \\
&- \left\langle(d J)_{p}\left(X_{t}\right) Z_{i}, \hspace{2.5em} Z_{j}\right\rangle \\
&= 0
.\end{align*}`{=tex}

**Claim**: This lemma immediately concludes the previous proof?

## Proof of Lemma

Extend $\left\{{Z_i}\right\}$ to a chart containing $p$ and use the Leibniz rule to rewrite

```{=tex}
\small
```
`\begin{align*}
- \left\langle J(p)\left(d X_{t}\right)_{p}\left(Z_{i}\right), Z_{j}\right\rangle 
+ \left\langle J(p)\left(d X_{t}\right)_{p}\left(Z_{j}\right), Z_{i}\right\rangle 
- \left\langle(d J)_{p}\left(X_{t}\right) Z_{i}, Z_{j}\right\rangle 
= 0
\end{align*}`{=tex} `\normalsize`{=tex} as `\footnotesize`{=tex} `\begin{align*}
&- \left\langle J\left(d X_{t}\right)\left(Z_{i}\right),Z_{j}\right\rangle 
+ \left\langle J\left(d X_{t}\right)\left(Z_{j}\right), Z_{i}\right\rangle
+ \left\langle J\left(d Z_{i}\right)\left(X_{t}\right), Z_{j}\right\rangle  
- {\color{red} \left\langle d\left(J Z_{i}\right)\left(X_{t}\right), Z_{j}\right\rangle } \\ \\
&=\left\langle J\left[X_{t}, Z_{i}\right], Z_{j}\right\rangle 
+ \left\langle J\left(d X_{t}\right)\left(Z_{j}\right), Z_{i}\right\rangle 
- {\color{red} \left\langle d\left(J Z_{i}\right)\left(X_{t}\right), Z_{j}\right\rangle }
.\end{align*}`{=tex} `\normalsize`{=tex}

where we'll rewrite the red terms.

## Proof of Lemma

```{=tex}
\scriptsize
```
Now use `\begin{align*}
X_t {\left\langle {JZ_i},~{Z_j} \right\rangle} = 0 
\implies
\left\langle d\left(J Z_{i}\right)\left(X_{t}\right), Z_{j}\right\rangle+\left\langle J Z_{i},\left(d Z_{j}\right)\left(X_{t}\right)\right\rangle=0
.\end{align*}`{=tex}

We now rewrite the RHS from before: `\begin{align*}
\left\langle J\left[X_{t}, Z_{i}\right], Z_{j}\right\rangle &+\left\langle J\left(d X_{t}\right)\left(Z_{j}\right), Z_{i}\right\rangle+\left\langle J Z_{i},\left(d Z_{j}\right)\left(X_{t}\right)\right\rangle \\ \\
&=\left\langle J\left[X_{t}, Z_{i}\right], Z_{j}\right\rangle+\left\langle J\left(d X_{t}\right)\left(Z_{j}\right)-J\left(d Z_{j}\right)\left(X_{t}\right), Z_{i}\right\rangle \\
&=\left\langle J\left[X_{t}, Z_{i}\right], Z_{j}\right\rangle-\left\langle J\left[X_{t}, Z_{j}\right], Z_{i}\right\rangle \\
&=\omega\left(\left[X_{t}, Z_{i}\right], Z_{j}\right)-\omega\left(\left[X_{t}, Z_{j}\right], Z_{i}\right)
.\end{align*}`{=tex}

The symmetry follows from $\omega$ being closed and `\begin{align*}
0
&= d \omega\left(X_{t}, Z_{i}, Z_{j}\right) \\
&= X_{t} \cdot \omega\left(Z_{i}, Z_{j}\right)-Z_{i} \cdot \omega\left(X_{t}, Z_{j}\right)+Z_{j} \cdot \omega\left(X_{t}, Z_{i}\right) \\
&\quad -\omega\left(\left[X_{t}, Z_{i}\right], Z_{j}\right)+\omega\left(\left[X_{t}, Z_{j}\right], Z_{i}\right)-\omega\left(\left[Z_{i}, Z_{j}\right], X_{t}\right) \\ \\
&= -X_{t} \cdot\left\langle Z_{i}, J Z_{j}\right\rangle+Z_{i} \cdot\left(d H_{t}\right)\left(Z_{j}\right)-Z_{j} \cdot\left(d H_{t}\right)\left(Z_{i}\right) \\
&\quad -\left(d H_{t}\right)\left(\left[Z_{i}, Z_{j}\right]\right)-\omega\left(\left[X_{t}, Z_{i}\right], Z_{j}\right)+\omega\left(\left[X_{t}, Z_{j}\right], Z_{i}\right) \\ \\
&= d\left(d H_{t}\right)\left(Z_{i}, Z_{j}\right)-\omega\left(\left[X_{t}, Z_{i}\right], Z_{j}\right)+\omega\left(\left[X_{t}, Z_{j}\right], Z_{i}\right) \\
&= -\omega\left(\left[X_{t}, Z_{i}\right], Z_{j}\right)+\omega\left(\left[X_{t}, Z_{j}\right], Z_{i}\right). \hspace{9em} \hfill\blacksquare
\end{align*}`{=tex}

# 8.4.6: Linearization of Hamilton's Equation

## Linearization of Hamilton's Equation

Recall `
<span class="math display">
\begin{align*}
\qty{d{\mathcal{F}}}_u = \mkern 1.5mu\overline{\mkern-1.5mu{\partial}\mkern-1.5mu}\mkern 1.5muY + SY = \qty{\mkern 1.5mu\overline{\mkern-1.5mu{\partial}\mkern-1.5mu}\mkern 1.5mu+ S}Y 
\end{align*}
<span>`{=html}

Now think of $S$ as a map $Y \mapsto S\cdot Y$, so $S\in C^\infty({\mathbb{R}}\times S^1; \endo({\mathbb{R}}^{2n}))$ and define the symmetric operators `
<span class="math display">
\begin{align*}
S^{\pm} \coloneqq\lim_{s\to \pm\infty} S(s, {-}) {\quad \operatorname{respectively} \quad}
\end{align*}
<span>`{=html}

Theorem
:   The equation `
    <span class="math display">
    \begin{align*}
    {\partial}_t Y = J_0 S^{\pm} Y
    \end{align*}
    <span>`{=html} is a linearization of Hamilton's equation `\begin{align*}
    {\frac{\partial z}{\partial t}\,} = X_t(z){\quad \operatorname{at} \quad} 
    \begin{cases}
    x = \lim_{s\to -\infty} u & \text{for } S^- \\
    y = \lim_{s\to \infty} u & \text{for } S^+
    \end{cases}\quad\text{respectively}
    .\end{align*}`{=tex}

## Proof

We first linearize Hamilton's equation at $x$: `\begin{align*}
{\frac{\partial z}{\partial t}\,} = X_t(z) \quad \stackrel{\text{linearized}}\implies \quad {\frac{\partial Y}{\partial t}\,} = (dX_t)_x Y
.\end{align*}`{=tex}

So write $Y = \sum y_i Z_i$ to obtain `\begin{align*}
\sum_{i} \frac{\partial y_{i}}{\partial t} Z_{i} &=\sum_{i} y_{i}\left(-\frac{\partial Z_{i}}{\partial t}+\left(d X_{t}\right)\left(Z_{i}\right)\right) \\
&=\sum_{i} \sum_{j} y_{i}\left\langle-\frac{\partial Z_{i}}{\partial t}+\left(d X_{t}\right)\left(Z_{i}\right), Z_{j}\right\rangle Z_{j} \\
&=\sum_{i} \sum_{j} y_{j}\left\langle-\frac{\partial Z_{i}}{\partial t}+\left(d X_{t}\right)\left(Z_{j}\right), Z_{i}\right\rangle Z_{i} \\ \\
\implies
\frac{\partial y_{i}}{\partial t}
&=\sum_{j}\left\langle-\frac{\partial Z_{j}}{\partial t}+\left(d X_{t}\right)\left(Z_{j}\right), Z_{i}\right\rangle y_{j}
.\end{align*}`{=tex}

## Proof

Thus we can rewrite the linearized equation as `\scriptsize`{=tex} `\begin{align*}
{\frac{\partial Y}{\partial t}\,} = (dX_t)_x Y = B^- \cdot Y, \quad 
b_{i j}=\left\langle-\frac{\partial Z_{j}}{\partial t}+\left(d X_{t}\right)_{x}\left(Z_{j}\right), Z_{i}\right\rangle
.\end{align*}`{=tex} `\normalsize `{=tex}

Recall `\scriptsize`{=tex} `\begin{align*}
A \coloneqq A\left(y_{1}, \ldots, y_{2 n}\right)=\sum y_{i}\left( {\color{red} J(u) \frac{\partial Z_{i}}{\partial t}-J(u)\left(d X_{t}\right)_{u}\left(Z_{i}\right) } \right)
.\end{align*}`{=tex} `\normalsize`{=tex}

Now take $s\to -\infty$ and look at the order zero part of $(d{\mathcal{F}})_u$. By the proof of 8.4.4, we have `\scriptsize`{=tex} `\begin{align*}
A\left(\sum y_{i} Z_{i}\right) &=\sum_{i}\left(J(x) \frac{\partial Z_{i}}{\partial t}-J(x)\left(d X_{t}\right)_{x}\left(Z_{i}\right)\right) \\
&=\sum_{i} \sum_{j} y_{i}\left\langle J \frac{\partial Z_{i}}{\partial t}-J\left(d X_{t}\right)\left(Z_{i}\right), Z_{j}\right\rangle Z_{j} \\
&=\sum_{i} \sum_{j} y_{j}\left\langle J \frac{\partial Z_{j}}{\partial t}-J\left(d X_{t}\right)\left(Z_{j}\right), Z_{i}\right\rangle Z_{i} \\
&=\sum_{i} \sum_{j}\left\langle-\frac{\partial Z_{j}}{\partial t}+\left(d X_{t}\right)\left(Z_{j}\right), J Z_{i}\right\rangle {y_{j}} Z_{i}
.\end{align*}`{=tex} `\normalsize`{=tex}

## Proof

Deduce that `\begin{align*}
S = (s_{ij}),\quad & s_{ij} = \left\langle-\frac{\partial Z_{j}}{\partial t}+\left(d X_{t}\right)_{x}\left(Z_{j}\right), ~~J(x) Z_{i}\right\rangle \\ \\ \\
JZ_i = \begin{cases}
Z_{i+n} & i \leq n \\
-Z_{i-n} & i \geq n+1
\end{cases}
&\implies 
s_{ij} = 
\begin{cases}
b_{i+n, j} & i \leq n \\
-b_{i-n, j} & i \geq n+1
\end{cases} \\ \\
&\iff S^- = - J_0 B^- 
.\end{align*}`{=tex} $\hfill\blacksquare$
