# Catalan

Website: <https://www.daniellitt.com/ccam>

[Link to book](<file:///home/zack/Dropbox/Library/Rene Schoof/Catalan's Conjecture (928)/Catalan's Conjecture - Rene Schoof.pdf>)

## Last Time

- The Diophantine equation $x^p-y^q = 1$ with $p, q\geq 2$ has only one 4-tuple solution: 
\[
(\pm 3)^2 - 2^3 = 1
.\]

- Used Mihăilescu's work from 2000-2003 to take care of odd prime cases.
  Leaves some cases:
  - $p=2$ with $q$ arbitrary,
  - $q=2$ with $p$ arbitrary,

- Reduced to elementary number theory!


## Today

- Today: the families
\[
x^2 - y^q = 1 && x^p - y^2 = 1
.\]

- Idea: prove 
  - $q=2$ and $p\geq 2$ arbitrary, 
  - $p=2$ and $q\geq 5$ arbitrary. 
  - Next time: $p=2, q=3$ in Chapter 4.
  Note $x^2 = y^3+1$ is an elliptic curve!
  Find solutions using descent (Raemeon!)

- Notation:
  - $\ord_p(x)$: the $p\dash$adic valuation of $x$.
  - $R^2$ for $R$ a ring: the set of squares in the ring (not the product!)
  - More generally: $R^p$ for the set of $p$th powers

### Preliminaries

:::{.lemma title="UFD Power Lemma"}
In $R$ a UFD, if $\gens{a, b} = \gens{1}$ and $ab = c^n \implies a = u_a r^n, b= u_b s^n$ for some units $u_a, u_b$ and $r,s \in R$.
:::

:::{.example title="?"}
Proof omitted, example has essential idea:

- $a = 2^8 3^4$,
- $b = 5^2 7^6$
- $c^2 = ab$, so $n=2$

Then write
\[
c^2 = ab = 2^8 3^4 5^2 7^6 = (2^4 3^2 5 7^3)^2 = (2^4 3^2)^2 (5 7^3)^2 \da r^2 s^2
.\]

Notes:

- $n$ had to divide every exponent
- For this, need coprimality: $n$ divided every exponent in the factorization of $c^2$, but this can go wrong by just splitting up a power:

  - $a= 2^8 3^4 5$
  - $b = 5 7^6$
:::

:::{.lemma title="Parity divisibility lemma"}
$1+i$ divides $a+bi$ in $\ZZ[i] \iff a,b$ have the same parity.
:::

:::{.proof title="of lemma"}
\envlist

- Use that $N(1+i) \divides N(\alpha) \iff (1+i)\divides \alpha$
  - $\impliedby$: Clear from properties of norm
  - $\implies$: Expand $a+bi = (1+i)(c + di)$ and solve a $2\times 2$ system.
- So $2\divides a^2 + b^2$, forcing them to have the same parity.

:::

:::{.lemma title="Exc 2.5"}
Extend \[
\ord_2:\ZZ&\to \ZZ_{\geq 0} \leadsto
\ord_2:\QQ\to \ZZ_{\geq 0}
\\ \\
\ord_2(x/y) &= \ord_2(x) - \ord_2(y) \\
\ord_2(0) &= \infty
.\]
Properties:
\[
\ord_2(xy)&= \ord_2(x) + \ord_2(y) \\
\ord_2(x+y) &\geq \min(\ord_2(x), \ord_2(y)) && \text{equality iff } \ord_2(x) \neq \ord_2(y)
.\]


:::

:::{.lemma title="Exc 3.2, GCD $q\dash$division lemma"}
For $q$ prime, $x,y\in \ZZ$ distinct with $\gcd(x, y) = 1$,
\[
\gcd\qty{ {x^q - y^q \over x-y}, x-y } \divides q
.\]


Note: useful because
\[
x^q - y^q = (x-y)\qty{x^q - y^q \over x-y}
.\]

:::


### Ch 2: $q=2$

\[
x^p - y^2 = 1
.\]

![](Projects/Current%20Projects/Catalan/figures/2021-09-10_01-16-59.png)

![](Projects/Current%20Projects/Catalan/figures/2021-09-10_01-18-12.png)

![](Projects/Current%20Projects/Catalan/figures/2021-09-10_01-18-33.png)

- Proof idea: a 2-adic argument, use properties of $\ZZ[i]$.

:::{.proposition title="2.1: V.A. Lebesgue, 1850"}
The Diophantine equation
\[  
x^p-  y^2 = 1
\]
has no solutions for $p\geq 2$ and $x, y\in \ZZ_{\neq 0}$.
:::

> Note: not Henri Lebesgue, of integral fame, late 1800s. Instead: Victor-Amédée Lebesgue, early 1880s. Simplified $n=4,5,7$ cases of Fermat's last theorem.


- Take $x, y$ nonzero solutions, so $x^p = y^2 + 1$.

:::{.claim}
Can assume $p$ is odd.
:::

:::{.proof title="of claim"}
\envlist

- If not, suppose $p$ is even.

- Factor
\[
(x^{p\over 2} - y)(x^{p\over 2} + y) = 1 \implies x^{p\over 2} \pm y = 1
,\]
where they both have to have the same sign.

- Subtract equations:
\[
x^{p\over 2} + y &= \pm 1\\
x^{p\over 2} - y &= \pm 1 \\
\hline \\
y-(-y) &= 0 \implies 2y = 0 \implies y=0
,\]

- But we assumed $y\neq 0$. 
  $\contradiction$

:::

:::{.claim}
$x, y$ have opposite parity.
:::

:::{.proof title="?"}
\envlist

- Reduce $\mod 2$.
- $y$ even $\implies y = 0 \mod 2 \implies y^2 = 0\mod 2 \implies x^p = y^2 + 1 = 1 \mod 2 \implies x$ odd
- $y$ odd $\implies y = 1 \mod 2 \implies y^2 = 1\mod 2 \implies x^p = y^2 + 1 = 1 + 1 = 2 = 0 \mod 2 \implies x$ even.


:::

:::{.claim}
$y$ is even, $x$ is odd. 
:::

:::{.proof title="of claim"}
\envlist

- Consider 
\[
x^p = y^2 + 1 \mod 4
.\]
- Consider all squares in $\ZZ/4$:
\[
\ZZ/4 = \ts{0,1,2,3} 
&\implies (\ZZ/4)^2 = \ts{0,1,4,9} = \ts{0,1,0,1} = \ts{0, 1} \\
&\implies y^2 = 0, 1\mod 4
.\]

- Toward a contradiction, suppose $y$ is odd (implicitly: $x$ is even)
- $y^2$ odd $\implies y^2 = 1,3 \mod 4 \implies y^2 = 1 \mod 4$ since the only squares mod 4 are 0, 1.
- Then $x^p = y^2 + 1 = 2\mod 4$.
- $x$ even $\implies x^n = 0 \mod 4$ for any $n \geq 2$.
  - Why: $x$ even $\implies x=0, 2 \mod 4 \implies x^2 = 0^2, 2^2 = 0 \mod 4$, etc.
- Now have $x^p = 2$ and $x^p = 0 \mod 4$. $\contradiction$


:::

:::{.claim}
$\gcd(1+iy, 1-iy) = 1 \in \ZZ[i]$.
:::

:::{.proof title="?"}
\envlist

- Check that $d\divides 1+iy \implies N(d) \divides 2$ so $N(d) = \pm 1,2$. 
- $N(d) = 1 \iff d$ is a unit
- $N(d) = 2 \iff a^2 + b^2 = 2 \implies a=b=1$
- $1+i \notdivides 1 \pm i y$ since $1, y$ have different parities, using that $y$ is even.

:::


- Since $p$ is odd, $U(\ZZ[i]) = \ts{\pm 1, \pm i}$ are all $p$th powers:
  - $(\pm 1)^p = \pm 1$
  - $i^p = \pm i \implies (-i)^p = -i^p = \mp i$.

- Factor
\[
x^p = y^2 + 1 &= (1+iy)(1-iy) \in (\ZZ[i])^p
.\]



Continuing the proof, use that $(1\pm iy)$ are coprime to apply UFD power lemma: 
\[
x^p = y^2 + 1 = (1+iy)(1-iy) &\in (\ZZ[i])^p \\
\implies 1 + iy &\in (\ZZ[i])^p && \text{by UFD lemma} \\
\implies 1 + iy &= c^p,\, \exists c\in \ZZ[i]
.\]

:::{.claim}
$c + \bar{c} = \pm 2$, and thus $c = \pm(1 + bi) \in 1 + i\ZZ$.
:::

:::{.proof title="?"}
Check
\[
c^p + \bar{c}^p = c^p + \bar{c^p} = (1+iy) + (1-iy) = 2
,\]

- Use that
\[
z^n - w^n 
&= (z-w)\sum_{k=0}^{n-1} z^kw^{n-k} \\
&= (z^{n-1} + z^{n-2}w + \cdots + w^{n-1}) \\ \\ 
\implies z^n + w^n &= z^n - (-w)^n && \text{for $n$ odd} \\
&= (z+w)\sum_{k=0}^{n-1} z^k(-w)^{n-k} \\
&= (z^{n-1} - z^{n-2}w + \cdots + w^{n-1}) && \text{since $n-1$ is even}
.\]

- Take $z= c^p, w=\bar{c}^p$:
\[
2 = c^p + \bar{c}^p 
&= (c+\bar c)(c^{p-1} - c^{p-2} \bar c + \cdots + \bar{c}^{p-1})
\\
\\
&\implies c+\bar c\divides 2 \in \ZZ \\
&\implies c+\bar c = \pm 2 \quad \text{ since } c + \bar{c} \text{ is even}
.\]

- Write $c = b'+ bi, \bar c= b' - bi$, then
\[
& \pm 2 = c + \bar c = 2b' \\
&\implies b' = \pm 1 \\
&\implies c = \pm(1 + bi)
.\]
:::

:::{.claim}
Since $y$ is even, $c = \pm(1 + bi)$ is not divisible by $1+i$. 
:::

:::{.proof title="of claim"}
Now WTS: $(1+i) \notdivides c$.

- Toward a contradiction: if so, 
\[
1+i &\divides c \\
\implies 1+i &\divides c^p = 1 + iy \\
\iff 1 &\equiv y \mod 2 && \text{by parity divisibility lemma}\\
\iff y &\text{ is odd} && \contradiction
.\]
:::

:::{.remark}
Now
\[
y \text{ even } &\implies (1+i)\notdivides c = \pm(1 + bi) \\
&\iff 1 \not\equiv b \mod 2 \quad \text{by parity divisibility lemma} \\
&\iff b \text{ is even} \\
&\implies c\in 1 + 2i\ZZ
.\]


- Now reduce $\mod 8$ to conclude that we take $+2$ in the following equation:
\[
\pm 2 = c^p + \bar{c}^p 
&= (1+bi)^p + (1-bi)^p \\
\implies 
\pm 2 &\equiv
(1+bi)^p + (1-bi)^p \mod 8\ZZ[i]
.\]


- Take binomial expansion of this expression to find a relation among the binomial coefficients ${p\choose k}$:
\[
{p \choose 2}(bi)^2 + {p\choose 4}(bi)^4 + \cdots + {p\choose p-1} (bi)^{p-1} = 0
.\]

:::

:::{.claim}
The leading term has the (strictly) **lowest** 2-adic valuation:
\[
S\da \sum s_k \da \ord_2\qty{ {p\choose k}(bi)^k } > \ord_2\qty{ {p\choose 2} (bi)^2 }
,\]
also implying that all of the pairs $(\ord_2(s_1), \ord_2(s_k))$ are distinct.
Thus
\[
\ord_2(S) = \min \ord_2(s_k) = \ord_2(s_1)
\]

:::

:::{.remark}
\envlist

- Why this finishes the proof: use that $\ord_2(a + b) \geq \min(\ord_2(a), \ord_2(b))$ with equality when $\ord_2(a)\neq \ord_2(b)$ are distinct.
- Note $S=0$, now apply above repeatedly to $s_1, s_k$ to get
\[
\ord_2(s_1) = \ord_2(S) = \ord_2(0) = 0\\
\implies \ord_2\qty{ {p\choose 2} (bi)^2 } = \ord_2\qty{{b^2p! \over 2(p-2)!} } = 0 \\
\implies b=0 \quad \text{since $b$ is even}
,\]

- Then
\[
c = 1+bi = 1+0i = 1 \\
\implies c=1 \\ \\
1 = c^p = 1+iy \\
\implies y=0
.\]

- This contradicts $y\in \ZZ_{\neq 0}$ and finishes the entire proof.
:::

:::{.proof title="?"}
\envlist

- WTS: $\ord(s_k/s_2) = \ord(s_k) - \ord(s_2) > 0$.
\[
\ord\qty{s_k\over s_2} &\da
\ord_2\qty{
{p\choose k} {p\choose 2}\inv (bi)^{k-2} 
}\\
&=
\ord_2\qty{ 
{p-2\choose k-2}\qty{2 (bi)^{k-2} \over k(k-1)}
}\\
&= \ord_2\qty{{p-2 \choose k-2}} + \ord_2\qty{2(bi)^{k-2}} - \ord_2(k(k-1)) \\
&> 0
,\]

- Use that 

  - Binomial coefficients are integers $\geq 1$ 
  - $b$ is even, 
  - $f(k) \da {\log(k) \over k-1}\searrow 0$, since $f'(k) < 0$ everywhere,
  - $f(2) = \log(2) \implies \log(2) > {\log k \over k- 1}$

- Then for any even $k\geq 4$,
\[
\ord_2( 2(bi)^{k-2} ) &\geq k-1 \\
&{\color{red}>} {\log k \over \log 2} \\
&\geq \ord_2(k) \\
&= \ord_2(k(k-1)) \quad \text{since $k-1$ is odd}\\
\implies &\ord_2(2(bi)^{k-2}) - \ord_2(k(k-1)) > 0
.\]

:::

### Ch. 3: $p=2$

\[
x^2 - y^q = 1 
.\]
![](Projects/Current%20Projects/Catalan/figures/2021-09-10_01-14-53.png)

![](Projects/Current%20Projects/Catalan/figures/2021-09-10_01-15-04.png)

![](Projects/Current%20Projects/Catalan/figures/2021-09-10_01-15-14.png)

![](Projects/Current%20Projects/Catalan/figures/2021-09-10_01-15-31.png)

- Proof due to Chao, 1965, adapted by Chein.
  
- Idea: for $q \geq 5$, we'll show $x^2-y^q=1$ has no solutions $x, y\in \ZZ_{\neq 0}$.
  - Toward a contradiction, we'll suppose such solutions exist.
  - Lemmas will give 
    - $x\equiv 0\mod q$ 
    - $x \equiv \pm 3 \mod q$ 
  - But since $q > 3$, this is absurd.

:::{.lemma title="3.1"}
For $q\geq 3 \in \ZZ$ an odd *integer* and $x^2-y^q=1$, we have

1. For some coprime $a, b$ with $\gcd(2a, b) = 1$,
  - $x-1 = 2^{q-1} a^q$
  - $x+1 = 2b^q$
  - $y=2ab$
2. $y\geq 2^{q-1}-2$.
:::


### Lemma 3.2

:::{.lemma title="3.2"}
For $q\geq 3 \in \ZZ$ an odd *prime* and $x^2-y^q=1$ for $x,y\in \ZZ_{\neq 0}$,
\[
x\equiv 0 \mod q
.\]
:::

- By contradiction: suppose
\[
x^2 = y^q + 1 && x,y\neq 0, x\not\equiv 0 \mod q
.\]
  We'll contradict $y\neq 0$.

- Write
\[
x^2 = y^q + 1 = (y+1)\qty{ y^q + 1 \over y+1}
,\]
noting typo in book.

:::{.claim title="Exercise 3.2"}
\[
d \da \gcd\qty{ y+1, \qty{ y^q + 1 \over y+1} } \implies d\divides q \implies d \in \ts{1, q}
.\]
:::

- Then $d\divides x^2$ but $x\not\equiv 0\mod q \implies d\neq q \implies d=1$.

:::{.claim title="Exercise 2.3"}
\[
y+1, \qty{ y^q + 1 \over y+1} \in \pm1 \cdot \ZZ^2 
.\]
:::

:::{.remark}
\envlist

- $y^q + 1 = x^2 \in \ZZ^2 \implies y\geq 0$ using that $q$ is odd.
  - If $y\leq -1$ then $y^q\leq -1 \implies y^q+1=x^2\leq -1, \contradiction$.
- $y\geq 0 \implies y+1 >0$ and ${y^q + 1\over y+1}>0$.
- $y+1>0$ and $y+1\in \pm1 \ZZ^2 \implies y+1 \in +1\ZZ^2 \implies y+1 = u^2$ for some $u\in \ZZ_{\neq 0}$.
- Consider solutions to 
\[
f(X, Y) \da X^2 -yY^2 = 1
.\]
  - Contains $(u, 1)$ since $u^2-y\cdot 1 = 1$
  - Contains $(x, y^{q-1\over 2})$ since $x^2 - y^q = 1$.

- $y\neq 0\implies y\geq 1$ is positive
- $y=u^2 -1 \geq 1$ is not a square (exercise) $\implies f$ is a **Pell equation**:

![$x^2-ny^2=1$ where $n$ is a nonsquare](Projects/Current%20Projects/Catalan/figures/2021-09-09_23-31-05.png)

- $y\not\in \ZZ^2 \implies \QQ[\sqrt y]/\QQ$ is quadratic and $\ZZ[\sqrt y] \leq \ZZ_K$ is a subring of its ring of integers
  - Note: $R \da \ZZ[\sqrt y]$ will be the ambient ring for the rest, with $\ZZ\dash$basis $\ts{1, \sqrt y}$.

- Exercise: $U(\ZZ[\sqrt y]) = \gens{-1. \eps \da u + \sqrt y}$ are generators of its unit group, treat them as a $\ZZ\dash$basis.

- Thus
\[
x + y^{q-1\over 2}\sqrt{y} = \pm(u + \sqrt y)^m,\quad \exists m\in \ZZ
.\]

- After possibly changing the sign of $u$, we can assume $m\geq 0$:
\[
(u + \sqrt y) \cdot -(-u + \sqrt y) = -(u^2 + y) = u^2 - y = 1 \\ 
\implies (u + \sqrt y)\inv = -(-u + \sqrt y)
.\]

- Reduce equation mod $y\ZZ[\sqrt y]$:
\[
x + {\color{red} y^{q-1\over 2}\sqrt{y} }  &\equiv \pm(u + \sqrt y)^m \mod yR \\
\implies 
x &\equiv \pm(u + \sqrt y)^m \mod yR \\
&\equiv \pm \sum_{k=0}^m {m\choose k}u^{m-k} (\sqrt y)^k \\
&\equiv \pm\qty{ u^m + {m\choose 1} u^{m-1}y^{1\over 2} + {m\choose 2}u^{m-2} y^1 + {\color{red} {m\choose 3}u^{m-3}y^{3\over 2} + \cdots} } \\
&\equiv \pm(u^m + mu^{m-1} y^{1\over 2}) \\
\implies
x &\equiv \pm(u^m + mu^{m-1} \sqrt y) \mod yR
.\]

- Now equate coefficients:
\[
mu^{m-1} \equiv 0 \mod yR \implies y\divides mu^{m-1}
.\]

:::

:::{.claim}
$y$ is even and $u$ is odd, since $y+1 = u^2$.
:::

- Proof: omitted.

:::{.remark}
\envlist

- Given this, since $y \divides mu^{m-1}$ with $y$ even and $u$ odd, $u^{\ell}$ is odd for all $\ell$, **so $m$ must be even.**

- $m$ even $\implies$ this is legal:
\[
x + y^{q-1\over 2}\sqrt y 
&= \pm (u + \sqrt y)^m \\
&= \pm\qty{\qty{u + \sqrt y}^2}^{m\over 2} \\
&= \pm \qty{u^2 + y + 2u\sqrt y }^{m\over 2} \\ \\
\implies 
x + y^{q-1\over 2}\sqrt y &\equiv \pm \qty{ {\color{red} u^2} + y + {\color{red} 2u\sqrt y} }^{m\over 2} \mod uR \\
&\equiv \pm y^{m\over 2} \\ \\
\implies x + y^{q-1\over 2}\sqrt y &\equiv \pm y^{m\over 2} + 0\sqrt y \mod uR \\
\implies u\divides y^{q-1\over 2}
.\]

- Now use $y+1 = u^2 \implies d\da \gcd(u, y) = 1$
  - Why: $d\divides y$ and $d\divides u$ implies $d\divides u^2$ and $d\divides u^2-y = 1$.

- Then $u\divides y^{q-1\over 2}$ and $\gcd(u, y ) = 1 \implies u = \pm 1$.

- Finish proof:
\[
y+1 = u^2 = (\pm 1)^2 = 1 \implies y=0, \contradiction
.\]

:::

### Lemma 3.3

:::{.lemma title="3.3"}
For $q\geq 3 \in \ZZ$ an odd *prime* and $x^2-y^q=1$,
\[
x\equiv \pm 3 \mod q
.\]
:::

- Trivial if $q=3$ since $\pm 3 \equiv 0\mod 3$ (applying previous lemma), so assume $q\geq 5$.


:::{.lemma title="3.1"}
Up to switching $x$ and $-x$,

\[
x-1 &= 2^{q-1} a^q\\
x+1 &= 2 b^q\\
y   &= 2ab \\
\gcd(a, b) = 1 &= \gcd(2a, b)
.\]
:::

Proof omitted.

- Use lemma to write
\[
(b^q)^2 - (2a)^q 
&= \qty{x+1\over 2}^2 - 2(x-1) \\
&= \qty{x^2 + 2x +1 - 8(x-1)\over 4} \\
&= \qty{x-3\over 2}^2
.\]

- Rewrite the LHS:
\[
(b^q)^2 - (2a)^q = (b^2 - 2a)\qty{ (b^2)^q - (2a)^q \over b^2 - 2a } \da \alpha_1 \alpha_2
.\]

- By the GCD $q\dash$division lemma (Exc. 3.2), 
\[
d\da \gcd( \alpha_1, \alpha_2)\divides q
\implies
d\in \ts{1, q}
.\]


:::{.claim}
\[
d=q
.\]

:::


:::{.remark}
Claim finishes the proof: 

- $q\divides d \implies q\divides \alpha_1$ and $q\divides \alpha_2$
- $\implies q\divides \alpha_1 \alpha_2 = \qty{x-3\over 2}^2$
- $\implies q\divides {x-3\over 2} \implies x\equiv 3 \mod q$.

:::

Proof of claim that $d=q$:

- Know $d\in \ts{1, q}$ so toward a contradiction suppose $d=1$ (we'll contradict this)
- Then $\alpha_1 \alpha_2\in \ZZ^2\implies \alpha_1, \alpha_2 \in \pm \ZZ^2$ (by previous lemma)
- Know 
\[
(b^2)^q - (2a)^q = \qty{x-3\over 2}^2 &\in +1\cdot \ZZ^2 \\
\implies
(b^2)^q &\geq (2a)^q \\
\implies b^2 &\geq 2a \\
\implies 
\alpha_1, \alpha_2 &> 0
.\]

- Also know $\alpha_1 = b^2-2a \in +1 \cdot \ZZ$ is a positive square

- $y\neq 0, y=2ab \implies a\neq 0$.

- Write $b^2 - 2a = c^2$ where $c^2\neq 0$ since $a\neq 0$.

- Now a contradiction: $\abs{a}\geq \abs{b}$ and $\abs{a} < \abs{b}$.

:::{.claim}
\[
\abs{a} \geq \abs{b}
.\]

:::


:::{.proof title="of claim"}
\envlist

- Closest squares to $b^2$ are $(b\pm 1)^2$, and
\[
\abs{(b\pm 1)^2 - b^2} 
&= \abs{ b^2 \pm 2b + 1 - b^2} \\
&= \abs{ 1 \pm 2b} \\
&\geq 2\abs{b} - \abs{1}
.\]
- Write $c^2 = b^2 - 2a$, then since $(b\pm 1)$ is the *closest* square:
\[
\abs{c^2 - b^2} \geq \abs{ (b\pm 1)^2 - b^2}\geq 2\abs{b} -1 \\
\implies
\abs{c^2 - b^2} = \abs{ (b^2 - 2a) - b^2} = \abs{2a} \geq 2\abs{b}-1 \\
\implies 2\abs{a} \geq 2\abs{b} - 1 \\ 
\implies \abs{a} \geq \abs{b}
,\]
since we're dealing with integers.
:::


:::{.claim}
\[
\abs{a} < \abs{b}
.\]
:::


:::{.proof title="of claim"}

\envlist

- Recall from lemma that $x+1 = 2b^q$
- Use $q\geq 5, q-1\geq 4, \abs x \geq 2$ to write
\[
\abs{a}^q &= {\abs {x-1} \over w^{q-1}} \\
&\leq {\abs{x-1} \over 2^4} \\
&< {\abs{x-1} \over 2} \\
&= {\abs{2b^q} \over 2} \\
&= \abs{b}^q
,\]
then take $q$th roots.
:::

This conclude the proof! $\contradiction$.


