# Monday, March 22

## 5.4: Spectral Sequence of a Filtration

:::{.remark}
We have an increasing filtration $F_p C \subseteq F_{p+1}C$, where we defined
\[
E_{p, q}^0 = { F_p C_{p+q} \over F_{p-1} C_{p+1} } &&
E_{p,q}^1 = H_{p+q} E_{p, *}^0
.\]

1. We have a map
  \[
  \eta_p: F_p C \surjects {F_p C \over F_{p-1}C } = E_p^0
  ,\]
  where we've dropped the $q$ from notation.

2. 
  \[
  A_{p, q}^r = \ts{ c \in C_p C \st dc \in F_{p-1} C } 
  ,\]
  the eventual cycles.
  We defined $Z_p^r = \eta_p A_p^r$ and $B_p^r = \eta_p dA_{p+r-1}^{r-1}$, and wrote $A_p^r \intersect F_{p-1}C = A_{p-1}^{r-1}$.

3. We had the chain of inclusions
\[
0 = B_p^r \subseteq \cdots \subseteq B_p^{\infty} \subset Z_p^{\infty } \subset \cdots \subseteq Z_p^1 = E_p^)
.\]

4. We also have $E_p^r = Z_p^r/B_p^r = A_p^r / dA_{p+r-1}^{r-1} + A_{p-1}^{r-1}$ 

5. $Z_{p}^{r+1}/B_pr \cong {A_p^{r+1} +A_{p-1}^{r-1} \over dA_{p+r-1} ^{r-1} + A_{p-1}^{r-1}}$.

6. $dA_p^r \intersect F_{p-r-1} C = dA_P^{r+1}$.

\todo[inline]{See video for missed spoken details!}

Obviously we have 
\[
d: A_p^r &\to A_{p-r}^{r} \\
d: A_{p-1}^r &\to dA_{p-1}^{r-1} 
,\]
so $d$ induces a well-defined map $d_p^r: E_p^r \mapsvia{} E_{p-r}^r$, which of course squares to zero, which goes $r$ columns to the left and decreases the total degree $n$ by 1 since the original $d$ did on $C_n$.
This is what we need to set up a spectral sequence, since we now have pages and differentials, and it just remains to show that $E^{r+1} \cong H_*(E^r, d^r)$.
:::

:::{.lemma title="?"}
$d$ determines isomorphisms $Z_{p}^r/Z_p^{r+1} \mapsvia{\sim} B_{p-r}^{r+1} / B_{p-r}^r$.
:::

:::{.proof title="?"}
Unwind definitions!
Note that we have $B_{p-r}^{r+1} = \eta_{p-r} dA_p^r$, using that the lower index on $B$ and upper index on $A$ should sum to the lower index on $A$.
This is equal to $dA_p^r / dA_p^r \intersect F_{p-r-1} C$, where the latter term is $\ker\eta_{p-r}$ and $B_{p-r}^r = \eta_{p-r} dA_{p-1}^{r-1}$.
This yields
\[
{B^{r+1}_{p-r} \over B_{p-r}^r}  
\cong 
{ dA_{p}^r \over dA_{p-1}^{r-1} + (dA_p^r \intersect F_{p-r-1} C) }
.\]
Similarly, 
\[
{Z_p^r \over Z_p^{r+1}} \da { \eta_p A_p^r \over \eta_p A_p^{r+1} } \cong {A_p^r \over A_p^{r+1} + (A_p^r \intersect F_{p-1} C )}
\congbecause{(3)} {A_p^r \over A_p^{r+1} + A_{p-1}^{r-1} }
.\]
Now applying the map induced by $d: A_p^r \to F_{p-r}C$ to this quotient, we have $\ker \ro{d}{A_p^r} \subseteq A_p^{r+1}$.
These go down $r$ steps, but everything in the kernel goes down as far as you'd like!
So $d$ kills one of the denominator terms, and thus induces an injective map on the quotient.
Thus \({Z_p^r \over Z_p^{r+1}} \mapsvia{\sim} {dA_p^r \over dA_p^{r+1} + dA_{p-1}^{r-1} } \), which is exactly the previous expression with the order switched, so this is isomorphic to $B_{p-r}^{r+1} / B_{p-r}^r$.
:::

:::{.proposition title="The $r+1$st page is the homology of the $r$th page"}
\[
{ \ker d_p^r \over \im d_{p+r}^r } \cong E_p^{r+1} \da {Z_p^{r+1} \over B_p^{r+1} }
.\]
:::

:::{.proof title="?"}
Recall that $d_p^r: E_p^r \to E_{p-r}^r$ and by (4), $E_p^r \cong {A_p^r \over dA_{p+r-1}^{r-1} + A_{p-1}^{r-1}}$.
Substituting $p \mapsfrom p-r$, we have
\[
\ker d_p^r = 
{
\ts{ z\in A_p^r \st dz \in dA_{p-1}^{r-1} + A_{p-r-1}^{r-1} } 
\over
dA_{p+r-1}^{r-1} + A_{p-1}^{r-1}
}
=
{
A_{p-1}^{r-1} + A_{p}^{r+1}
\over 
dA_{p+r-1}^{r-1} + A_{p-1}^{r-1}
}
\congbecause{(5)}
{Z_p^{r+1} \over B_p^r} && \text{which is } (6)
.\]
Here we've used that $x\in F_p C\implies dx \in F_{p-r-1} C \implies dx\in A^{?}_{p-r-1}$.
What is the image of $d_p^r$ in general?
Note that later we can replace $p\mapsfrom p+r$.
By the 1st isomorphism theorem, we have
\[
d_p^r: E_p^r = Z_p^r / B_p^r \mapsvia{\sim} {Z_p^r / B_p^r \over Z_p^{r+1} / B_p^r} \mapsvia{\sim} {Z_p^r \over Z_p^{r+1}} \mapsvia{d} 
{B_{p-r}^{r+1} \over B_{p-r}^r} \injects {Z_{p-r}^r \over B_{p-r}^r} = E_{p-r}^r
,\]
where we've applied the lemma from last time, and we've used the fact that in the last map, all of the $B$ are contained in all of the $Z$, so we can choose any superscript we want.
These are all isomorphisms up until the last part, so 
\[
\im d_p^r \cong B_{p-r}^{r+1} / B_{p-r}^{r+1}
.\].
Replacing $p\mapsfrom p+r$, we get a 7th fact


:::{.fact title="7"}
\[
\im d_{p+r}^r \cong B_{p}^{r+1} / B_{p}^{r+1}
.\]
:::

Now combining (6) and (7), we have 
\[
{\ker d_p^r \over \im d_{p+r}^{r} } \mapsvia{\sim} {Z_p^{r+1} / B_p^r \over B_{p}^{r+1} / B_p^r } \cong {Z_p^{r+1} \over B_p^{r+1}} = E_p^{r+1}
.\]

:::

## 5.5: Convergence of the Spectral Sequence of a Filtration

:::{.remark}
We'll restrict our attention to bounded complexes.
:::

:::{.remark}
A filtration $F$ on a chain complex $C$ induces a filtration on the homology $H_*C$,
where $H_p H_n C = \im ( H_n F_p C \to H_n C)$:

\begin{tikzcd}
	{F_p C_{n+1}} && {C_{n+1}} \\
	\\
	{F_p C_{n}} && {C_{n}} \\
	\\
	{F_p C_{n-1}} && {C_{n-1}}
	\arrow[hook, from=1-1, to=1-3]
	\arrow[hook, from=3-1, to=3-3]
	\arrow[hook, from=5-1, to=5-3]
	\arrow["d"{description}, from=1-1, to=3-1]
	\arrow["d"{description}, from=3-1, to=5-1]
	\arrow["d"{description}, from=1-3, to=3-3]
	\arrow["d"{description}, from=3-3, to=5-3]
\end{tikzcd}

> [Link to Diagram](https://q.uiver.app/?q=WzAsNixbMCwwLCJGX3AgQ197bisxfSJdLFsyLDAsIkNfe24rMX0iXSxbMiwyLCJDX3tufSJdLFsyLDQsIkNfe24tMX0iXSxbMCwyLCJGX3AgQ197bn0iXSxbMCw0LCJGX3AgQ197bi0xfSJdLFswLDEsIiIsMCx7InN0eWxlIjp7InRhaWwiOnsibmFtZSI6Imhvb2siLCJzaWRlIjoidG9wIn19fV0sWzQsMiwiIiwwLHsic3R5bGUiOnsidGFpbCI6eyJuYW1lIjoiaG9vayIsInNpZGUiOiJ0b3AifX19XSxbNSwzLCIiLDAseyJzdHlsZSI6eyJ0YWlsIjp7Im5hbWUiOiJob29rIiwic2lkZSI6InRvcCJ9fX1dLFswLDQsImQiLDFdLFs0LDUsImQiLDFdLFsxLDIsImQiLDFdLFsyLDMsImQiLDFdXQ==)

\todo[inline]{See video for missed details.}

These inclusions induce a map from the homology of the subcomplex to the homology of the total complex.
:::

:::{.remark}
If the filtration on $C$ is bounded, say $0 = F_s C_n \subseteq \cdots \subseteq F_t C_n = C_n$ for some $s<t$, then so is the induced filtration on $H_n C$.
Also note that $F_t H_n = H_n$ and $F_s H_n = 0$.
:::

:::{.theorem title="Classical Convergence Theorem"}
Assume $F$ is a bounded filtration on $C$, then the spectral sequence is bounded and converges to $H_*C$, so
\[
E^1_{p, q} = H_{p+q}\qty{ F_p C \over F_{p-1} C } \abuts H_{p+q}C
.\]
:::

:::{.remark}
Need to check next time that the $E^{\infty }_{p, q}$ terms give the proper quotients.
:::


