# Wednesday, November 18



## Steinberg Tensor Product Formula

Recall the Steinberg tensor product formula:
Let $\lambda \in X(T_+)$ with $\ch(k) = p$, then write
\[  
\lambda = \sum_{j=1}^s p^j \lambda_j
\]
with $\lambda_j \in X_1(T)$.
Then
\[  
L(\lambda) = L(\lambda_0) \tensor \bigotimes_{j=1}^s L(\lambda_j)^{(j)}
.\]

The goal is to find a formula resembling this for $G$ and $G_r\dash$modules.

:::{.proposition title="?"}
Let $\lambda_0 \in X_r(T), \lambda_1 \in X(T)$.
Then there exists an isomorphism of $G_r T\dash$modules
\[  
\hat{Q}_{r+1} (\lambda_0 + p^r \lambda_1) = \hat{Q}_r (\lambda_0) \tensor \hat{Q}_1(\lambda_1)^{(r)}
,\]
and by inflation, $\hat{Q}_1(\lambda)^{(r)}$ is a $G_r T\dash$module.
:::

:::{.proof title="?"}
We have a decomposition of $G_r T\dash$modules:
\[  
\soc_{G_r} \hat{Q}_{r+1}(\lambda) = \bigoplus_{\mu\in X_r(T)} \hat{L}_r(\mu) \tensor \Hom_{G_r}(\hat{L}_r(\mu), \hat{Q}_{r+1}(\lambda) )
.\]

We can write

\[  
\soc_{G_{r+1}} \hat{Q}_{r+1}(\lambda) 
&= \hat{L}_{r+1}(\lambda) \\
&= \hat{L}_r(\lambda_0) \tensor \hat{L}_1(\lambda_1)^{(r)}
.\]
And since there can only be one summand, we can combine these two to write

\[  
\soc_{G_r} \hat{Q}_{r+1}(\lambda) = \hat{L}_r(\lambda_0) \tensor \Hom_{G_r}(\hat{L}_r(\lambda_0), \hat{Q}_{r+1}(\lambda) )
,\]
which implies that 
\[  
\soc_{G_{r+1} T} \hom_{G_r}(\hat{L}_r(\lambda_0), \hat{Q}_{r+1}(\lambda)  ) &\cong \hat{L}_1(\lambda_1)^{(r)}
.\]

We want to show that this hom is injective, so we'll use the Lydon-Hochschild-Serre spectral sequence
\[  
E_2^{i, j} = \Ext_{G_{r+1} T/G_r}^i (N, \ext^j( \hat{L}_r(\lambda_0), \hat{Q}_{r+1}(\lambda) )  )
\abuts
\ext^{i+j}_{G_{r+1} T} ( N\tensor \hat{L}_r(\lambda_0), \hat{Q}_{r+1}(\lambda) )
.\]

There will be a lot of vanishing here.
We know that

- $\hat{Q}_{r+1}(\lambda)$ is an injective $G_{r+1}T\dash$module, and
- $\hat{Q}_{r+1}(\lambda)$ is an injective $G_{r}\dash$module,

so $E_2^{>0, 0} = 0$:

\[  
\ext_{G_{r}T/G_r}^i(N, \Hom_{G_r}( \hat{L}_r(\lambda_0), \hat{Q}_{r+1}(\lambda) )  )
.\]

We can thus conclude that $\hom_{G_r}( \hat L_r(\lambda_0), \hat Q_{r+1}(\lambda) )$ is an injective $G_{r+1}T/G_r\dash$module.
Thus
\[  
\Hom_{G_r}(\hat L_r(\lambda_0), \hat Q_{r+1}(\lambda) ) \cong \hat Q_{1}(\lambda_1)^{(r)}
.\]

To finish the proof, note that $\hat{Q}_{r+1}(\lambda) \downarrow_{G_r T} = \bigoplus_{j=1}^m \hat{Q}_r(\mu_j)$, and thus
\[  
\hat{Q}_{r+1}(\lambda) = \bigoplus_{j-1}^m \hat{Q}_r(\lambda_0) \tensor p^r v_j
.\]

Furthermore, at the level of characters we have $\sum e^{v_j} = \ch \hat Q_1(\lambda_1)$ and thus
\[  
\hat Q_1(\lambda_1)^{(r)} = \bigoplus_{j=1}^m p^r v_j
.\]
:::

:::{.remark}
Suppose $\lambda_0, \lambda_1, \lambda_{r-1}\in X(T)$, where we can write $\lambda = \sum_{i=0}^{r-1} \lambda_i p^i$.
Then for characters we have
\[  
\hat Q_{r}(\lambda) = \prod_{j=0}^{r-1} \ch \hat{Q}_1(\lambda_j)^{(j)}
.\]
:::

Let $L(\lambda)$ be an irreducible representation for $G$, and set $Q_\lambda$ to be the injective hull of $L(\lambda)$, so we have an exact sequence $0 \to L(\lambda) \injects Q(\lambda)$.

:::{.proposition title="?"}
Let $\lambda\in X_r(T)$, and assume that the $G_r T\dash$ structure on $\hat Q_r(\lambda)$ can be lifted to $G$.
Then

a. If $\lambda'\in X(T)_+$, then there exists an isomorphism of $G\dash$modules:
\[  
\hat{Q}_r(\lambda) \tensor Q_{\lambda'}^{(r)} \cong Q_{\lambda + p^r \lambda'}
.\]

b. If $\lambda'\in X(T)$ and $r'>r$, then there exists an isomorphism of $G_{r'} T\dash$modules
\[  
\hat Q_r(\lambda) \tensor \hat Q_{r' - r}(\lambda')^{(r)} \cong \hat Q_{r'}(\lambda + p^r \lambda')
.\]

:::


:::{.proof title="of a"}
We want to show that $\hat Q_r(\lambda) \tensor Q_{\lambda'}^{(r)}$ is an injective $G\dash$module and that the socle of the LHS is equal to $L(\lambda + p^r \lambda')$.

:::{.claim}
Let $N\normal G$ be groups, and suppose $V_1 \in \mods{G}$ is injective as an $N\dash$module and $V_2$ is injective as a $G/N\dash$module.
Then $V_1 \tensor V_2$ is injective as a $G\dash$module.
:::

:::{.proof title="of claim"}

We'll again use the LHS spectral sequence,
\[  
E_{2}^{i, j} = \ext_{G/N}^i(k, \ext_N^j(E, V_1\tensor V_2) )
\abuts
\Ext_G^{i+j}(E, V_1 \tensor V_2)
.\]
Using the assumption that $V_1$ is injective as an $N\dash$module, we have collapsing
\[  
\ext_N^{>0}(E, V_1\tensor V_2) = \ext_N^{>0} (E\tensor V_2, V_1)
.\]
and thus
\[  
\ext_{G/N}^{>0}(k, \Hom_N(E, V_1\tensor V_2) )
= \Ext_G^{>0}(N, V_1\tensor V_2)
= 0
.\]
For the first line, we can write $\hom_N(E, V_1) \tensor V_2$.
This vanishes for every possible $E$, making $V_1\tensor V_2$ injective.
:::

In our situation, we'll be taking $N\da G_r \normal G$, where $G/G_r = G^{(r)}$.
Thus the claim proves part (a).
:::

:::{.proof title="of b"}
Recall that the $G\dash$socle is contained in $\soc_{G_r}$, yielding
\[  
\soc_{G_r} \hat Q_r(\lambda) \tensor Q_{\lambda'}^{(r)} 
= \hat L_R(\mu) \tensor \Hom_{G_r}( \hat L_r(\mu), \hat Q_r(\lambda)  ) \tensor Q_{\lambda}^{(r)}
.\]
We know that the hom is only nonzero when $\lambda = \mu$, so this is equal to
\[  
\cdots
&= \hat{L}_R(\lambda) \tensor Q_{\lambda'}^{(r)}
,\]
since in this term, the hom is just equal to $k$.
Thus we have
\[  
\soc_G \hat Q_r(\lambda) \tensor Q_{\lambda'}^{(r)}
= \hat L_r(\lambda) \tensor L(\lambda')^{(r)} = \soc_G Q_{\lambda+ p^r \lambda'}
.\]
Since this is an injective module and the socles match, this must be an isomorphism.
:::

:::{.corollary title="?"}
Let $\lambda \in X(T)_+$ with $\lambda = \sum_{j=0}^s \lambda_j p^j$ with $\lambda_j \in X_1(T)$.
Moreover, assume all $Q_r(\mu)$ lift to $G$.
Then there exists a $\mods{G}$ isomorphism
\[  
Q_r(\lambda) = \bigotimes_{j=0}^s \hat Q_1(\lambda_j)^{(j)}
.\]
:::

Next time: cohomology of Frobenius kernels and relation to the nilpotent cones, related to ABG equivalence, computing the cohomology ring for $G_1$.
