# Friday, September 18

## Frobenius Kernels

Let $\ch(k)  p > 0$ and let $G$ be an algebraic group scheme.
We have a Frobenius map  $F:G\to G$ given by $F((x_{ij})) = (x_{ij}^p)$, which we can iterate to get $F^r$ for $r\in \NN$.
Setting $G_r = \ker F^r$ the $r$th Frobenius kernel, we get a normal series of group schemes
\[  
G_1 \normal G_2 \normal \cdots \normal G
.\]

There is an associated chain of finite dimensional Hopf algebras
\[  
\Dist(G_1) \leq \Dist(G_2) \leq \cdots \leq \Dist(G)
.\]

Then $k[G]\dual = \Dist(G_r)$, and we get an equivalence of representations for $G_r$ to representations for $\Dist(G_r)$.

A special case will be when $G$ is a reductive algebraic group scheme.
We'll start by finding a basis for $\Dist(G_r)$.

Recall the PBW theorem: we have a basis for $\lieg$ given by
\[  
\ts{x_\alpha \st \alpha\in \Phi^+ } &\text{ Positive root vectors} \\
\ts{h_i \st i=1,\cdots, n} &\text{ A basis for } t \\
\ts{x_\alpha \st \alpha\in \Phi^- } &\text{ Negative root vectors} \\
.\]

We can then obtain a basis for $U(\lieg)$:
\[  
U(\lieg) = \gens{ \prod_{\alpha\in\Phi^+} x_\alpha^{n(\alpha)} \prod_{i=1}^n h_i^{k_i} \prod_{\alpha\in\Phi^+} x_{-\alpha}^{m(\alpha)}  }
.\]

We can similarly obtain a basis for the distribution algebra
\[  
\Dist(G) = \gens{ 
\prod_{\alpha\in\Phi^+} { x_{\alpha}^{n(\alpha)} \over n!} 
\prod_{i=1}^n {h_i \choose k_i} 
\prod_{\alpha\in\Phi^+} { x_{-\alpha}^{n(\alpha)} \over n!} 
}
,\]
and we can similar get $\Dist(G_r)$ by restricting to $0\leq n(\alpha), k_i, m(\alpha) \leq p^r - 1$.
Above the $k_i$ are allowed to be any integers.
This yields a triangular decomposition
\[  
\Dist(G_r) = \Dist(U_r^+) \Dist(T_r) \Dist(U_r^-)
,\]
where we'll denote the first two terms $\Dist(B_r^+)$ and the last two as $\Dist(B_r)$.

## Induced and Coinduced Modules

Goal:
Classify simple $G_r\dash$modules.
We know the classification of simple $G\dash$modules, so we'll follow similar reasoning.
We started by realizing $L(\lambda) \injects \ind_B^G \lambda$ as a submodule (the socle) of some "universal" module.

Let $M$ be a $B_r\dash$module, we can then define 
\[  
\ind_{B_r}^{G_r}M = \qty{k[G_r] \tensor M }^{B_r}
,\]
where we're now taking the $B_r\dash$invariants.
We get a decomposition as vector spaces,
\[  
k[G_r] = k[U_r^+] \tensor_k k[B_r]
\]
and thus an isomorphism
\[  
\ind_{B_r}^{G_r}M = \qty{k[G_r] \tensor M }^{B_r} 
\cong k[U_r^+] \tensor \qty{ k[B_r] \tensor M}^{B_r}
\cong k[U_r^+] \tensor M
\]
since $k[B_r]\tensor M \cong \ind_{B_r}^{B_r} M \cong M$.

We then define
\[  
\coind_{B_r}^{G_r} = \Dist(G_r) \tensor_{\Dist(B_r)} \tensor M
,\]
which is an analog of $U(\lieg)\tensor_{U(\lieb)} M$.

We have $\Dist(U_r^+) \tensor \Dist(B_r) \cong \Dist(G_r)$, so

\[  
\coind_{B_r}^{G_r} = \Dist(G_r) \tensor_{\Dist(B_r)} \tensor M
\cong
\Dist(U_r^+) \tensor_k \Dist(B_r) \tensor_{\Dist(B_r)} M 
\cong
\Dist(U_r^+) \tensor_k M
,\]
which we'll define as the **coinduced module**.

We can compute the dimension:
\[  
\dim \ind_{B_r}^{G_r} M = \dim \coind_{B_r}^{G_r} M = \qty{\dim M} p^{r\abs{\Phi^+}}
.\]

> Open: don't know how to compute composition factors.

:::{.proposition title="?"}
\hfill

1. \[\coind_{B_r}^{G_r} M \equiv \ind_{B_r}^{G_r} M\tensor 2(p^r - 1)\rho,\] where the last term is a one-dimensional $B_r\dash$module and $\rho$ is the *Weyl weight*.

2. \[\coind_{B_r^+}^{G_r} M \cong \ind_{B_r^+}^{G_r} M \tensor -2\qty{p^r-1}\rho\]

where
\[  
\rho = {1\over 2}\sum_{\alpha\in\Phi^+} \alpha = \sum_{i=1}^n w_i
.\]
:::


:::{.proof title="Sketch for (1)"}
Since the tensor product satisfies a universal property, we have a map
\begin{center}
\begin{tikzcd}
M \ar[rd, "B_r"]\ar[rr] & & \Dist(G_r)\tensor_{\Dist(B_r)} M\ar[dl, "\exists \psi", dotted] \\
& N = M\ind_{B_r}^{G_r} \tensor 2(p^r-1)\rho &
\end{tikzcd}
\end{center}

1. We need to find a $B_r$ morphism $f:M\to N$.

2. We need to show that $f$ generates $N$ as a $G_r\dash$module.


Note that if (1) and (2) hold, then  $\psi$ is surjective, but since $\dim \coind_{B_r}^{G_r} M= \dim N$ this forces $\psi$ to be an isomorphism.

We can write
\[  
\ind_{B_r}^{G_r} M\tensor 2(p^r-1) \rho
&=
\qty{ k[G_r] \tensor M \tensor 2(p^r-1) \rho  }^{B_r} \\
&\cong
\hom_{B_r}\qty{\Dist(G_r), M\tensor 2(p^r-1)\rho }
.\]

Let $g_m(x) \da m\tensor 2(p^r-1)\rho$ for any $x =\prod_{\alpha\in\Phi^+} {x_\alpha^{p^r-1} \over \qty{p^r-1}! }$, and $g_m(x) = 0$ for any other $x$.

Now define $f(m) = g_m$, and check that $\im f$ generates $N$.
:::

## Verma Modules

Recall that $W(\lambda) \da U(\lieg) \tensor_{U(\lieb^+)} \lambda$ were the *Verma modules* for lie algebras.

Let $\lambda \in X(T)$, we have $T_r \leq T$ and restriction yields a map $X(T) \to X(T_r)$.
Given a weight $\lambda$,  we can write it $p\dash$adically as
\[  
\lambda = \lambda_0 + \lambda_1 p + \lambda_2 p^2 + \cdots + \lambda_{r-1} + \cdots
.\]

This yields an exact sequence
\[  
0 \to p^r X(T) \to X(T) \to X(T_r) \to 0
,\]

and thus $X(T) / p^r X(T) \cong X(T_r)$.

Let $\lambda \in X(T_r)$, then $\lambda$ becomes a $B_r\dash$module by letting $U_r$ act trivially, since we have 
\[  
\cdots U_r \to B_r \surjects T_r \to 0
.\]

Set $Z(r) = \coind_{B_r}^{G_r} \lambda$, and set $Z(r)' = \ind_{B_r}^{G_r} \lambda$.
Then $\dim Z_r(\lambda) = \dim Z_r'(\lambda) = p^{r\abs{\Phi^+}}$.
We'll then think of 

- $\coind \surjects L_r(\lambda)$ being in the head,
- $L_r(\lambda) \injects \ind$ being the socle.

> Note that the dimensions aren't known, nor are the projective covers or injective hulls.

We have a form of translation invariance, namely
\[  
Z_r(\lambda + p^r\nu) = Z_r(\lambda) \qquad &\forall \nu \in X(T) \\
Z_r'(\lambda + p^r\nu) = Z_r'(\lambda) \qquad &\forall \nu \in X(T)
.\]

:::{.proposition title="?"}
Let $\lambda \in X(T)$.

1. $Z_r(\lambda){\downarrow}_{B_r}$ is the projective cover of $\lambda$ and the injective hull of $\lambda - 2(p^r-1)\rho$.
2. $Z_r'(\lambda){\downarrow}_{B_r^+}$ is the injective hull of $\lambda$ and the projective hull of $\lambda - 2(p^r-1)\rho$.

:::


